src/BinEncoders/Env/Automation/Solver.v
@@ -5,6 +5,7 @@ Require Import
         Fiat.Common.BoundedLookup
         Fiat.Common.ilist
         Fiat.Common.Tactics.CacheStringConstant
+        Fiat.Common.IterateBoundedIndex
         Fiat.Computation
         Fiat.QueryStructure.Specification.Representation.Notations
         Fiat.QueryStructure.Specification.Representation.Heading
@@ -14,13 +15,16 @@ Require Import
         Fiat.BinEncoders.Env.Common.WordFacts
         Fiat.BinEncoders.Env.Common.ComposeIf
         Fiat.BinEncoders.Env.Common.ComposeOpt
+        Fiat.BinEncoders.Env.Lib2.Option
         Fiat.BinEncoders.Env.Lib2.FixListOpt
+        Fiat.BinEncoders.Env.Lib2.Bool
         Fiat.BinEncoders.Env.Lib2.NoCache
         Fiat.BinEncoders.Env.Lib2.WordOpt
         Fiat.BinEncoders.Env.Lib2.NatOpt
         Fiat.BinEncoders.Env.Lib2.Vector
         Fiat.BinEncoders.Env.Lib2.EnumOpt
         Fiat.BinEncoders.Env.Lib2.SumTypeOpt
+        Fiat.BinEncoders.Env.Lib2.StringOpt
         Fiat.BinEncoders.Env.Common.Sig
         Fiat.BinEncoders.Env.BinLib.FixInt
         Fiat.BinEncoders.Env.BinLib.Char
@@ -104,6 +108,76 @@ Ltac build_fully_determined_type :=
   (* Substitute any inferred equalities *) subst;
   (* And unify with original object *) reflexivity.
 
+  Lemma decides_True' {A}
+    : forall a, decides true ((fun _ : A => True) a).
+  Proof.
+    simpl; intros; exact I.
+  Qed.
+
+Definition pair_eq_dec {A B}
+      (A_eq_dec : forall a a' : A, {a = a'} + {a <> a'})
+      (B_eq_dec : forall a a' : B, {a = a'} + {a <> a'})
+  : forall a a' : A * B, {a = a'} + {a <> a'}.
+Proof.
+  refine (fun a a' => match A_eq_dec (fst a) (fst a'), B_eq_dec (snd a) (snd a') with
+                      | left _, left _ => _
+                      | _, _ => _
+                      end);
+    decide equality.
+Defined.
+
+Definition decides_pair_eq {A B}
+           (t : A -> A -> bool)
+           (t' : B -> B -> bool)
+           (decides_t : forall a a' : A , decides (t a a') (a = a'))
+           (decides_t' : forall b b' : B , decides (t' b b') (b = b'))
+  : forall ab ab' : A * B,
+    decides (andb (t (fst ab) (fst ab')) (t' (snd ab) (snd ab'))) (ab = ab').
+Proof.
+  destruct ab; destruct ab'; simpl in *.
+  pose proof (decides_t a a0);   pose proof (decides_t' b b0);
+    unfold decides, If_Then_Else in *.
+  destruct (t a a0);  destruct (t' b b0); simpl in *; congruence.
+Qed.
+
+Lemma decides_nat_eq :
+  forall (n n' : nat),
+    decides (EqNat.beq_nat n n') (n = n').
+Proof.
+  unfold decides, If_Then_Else; intros.
+  destruct (EqNat.beq_nat n n') eqn: ? ;
+    try eapply EqNat.beq_nat_true_iff;
+    try eapply EqNat.beq_nat_false_iff; eauto.
+Qed.
+
+Lemma decides_word_eq {sz}:
+  forall (w w' : word sz),
+    decides (weqb w w') (w = w').
+Proof.
+  unfold decides, If_Then_Else; intros.
+  destruct (weqb w w') eqn: ? ;
+    unfold not; setoid_rewrite <- weqb_true_iff; congruence.
+Qed.
+
+Lemma decides_bool_eq :
+  forall (b b' : bool),
+    decides (eqb b b') (b = b').
+Proof.
+  unfold decides, If_Then_Else; intros;
+    destruct b; destruct b'; simpl; congruence.
+Qed.
+
+Lemma decides_EnumType_eq {A} {n} {tags} :
+  forall (b b' : @EnumType n A tags),
+    decides (fin_beq b b') (b = b').
+Proof.
+  unfold decides, If_Then_Else; intros.
+  destruct (fin_beq b b') eqn: H' ;
+    unfold not; intros;
+      try rewrite fin_beq_dec in H';
+      try rewrite fin_beq_neq_dec in H'; eauto.
+Qed.
+
 Ltac decide_data_invariant :=
   (* Show that the invariant on the data is decideable. Most *)
   (* of the clauses in this predicate are obviously true by *)
@@ -111,36 +185,154 @@ Ltac decide_data_invariant :=
   (* by a decision procedure*)
   unfold GetAttribute, GetAttributeRaw in *;
   simpl in *; intros; intuition;
-  repeat
-    first [ progress subst
+    repeat first [ progress subst
+             | match goal with
+                 |- decides ?A (?B ?C)  =>
+                 let T := type of C in
+                 unify B (fun _ : T => True);
+                 apply (@decides_True' T C)
+               end
           | apply decides_eq_refl
           | solve [eauto with decide_data_invariant_db]
           | eapply decides_and
           | eapply decides_assumption; eassumption
-          | eapply decides_dec_eq; auto using Peano_dec.eq_nat_dec, weq ].
+          | apply decides_dec_lt
+          | eapply decides_word_eq
+          | eapply decides_nat_eq
+          | eapply decides_pair_eq
+          | eapply decides_bool_eq
+          | eapply decides_EnumType_eq
+          | eapply decides_dec_eq; auto using Peano_dec.eq_nat_dec, weq, pair_eq_dec ].
+
+Ltac ilist_of_evar B As k :=
+  match As with
+  | VectorDef.nil _ => k (@inil _ B)
+  | VectorDef.cons _ ?a _ ?As' =>
+    makeEvar (B a)
+             ltac:(fun b =>
+                     ilist_of_evar
+                       B As'
+                       ltac:(fun Bs' => k (icons (l := As') b Bs')))
+  end.
+
+Ltac Vector_of_evar n T k :=
+  match n with
+  | 0 => k (@Vector.nil T)
+  | S ?n' => Vector_of_evar
+               n' T
+               ltac:(fun l =>
+                       makeEvar
+                         T
+                         ltac:(fun a => k (@Vector.cons T a n' l)))
+  end.
 
 Ltac decode_step :=
   (* Processes the goal by either: *)
   match goal with
+  | |- appcontext [encode_decode_correct_f _ _ _ _ ?H _ _] =>
+    progress unfold H
+  | |- appcontext [encode_unused_word_Spec] =>
+      unfold encode_unused_word_Spec
   (* A) decomposing one of the parser combinators, *)
   | |- _ => apply_compose
   (* B) applying one of the rules for a base type  *)
-  | |- appcontext [encode_decode_correct_f _ _ _ _ (encode_Vector_Spec _) _ _] =>
-    intros; eapply Vector_decode_correct
   | H : cache_inv_Property _ _
     |- appcontext [encode_decode_correct_f _ _ _ _ encode_word_Spec _ _] =>
     intros; revert H; eapply Word_decode_correct
+  | |- appcontext [encode_decode_correct_f _ _ _ _ (encode_unused_word_Spec' _ _) _ _] =>
+    let H := eval simpl in unused_word_decode_correct in
+        apply H
+
+  | |- appcontext [encode_decode_correct_f _ _ _ _ (encode_Vector_Spec _) _ _] =>
+    intros; eapply Vector_decode_correct
+
   | |- appcontext [encode_decode_correct_f _ _ _ _ encode_word_Spec _ _] =>
     eapply Word_decode_correct
   | |- appcontext [encode_decode_correct_f _ _ _ _ (encode_nat_Spec _) _ _] =>
     eapply Nat_decode_correct
+  | |- appcontext [encode_decode_correct_f _ _ _ _ (encode_list_Spec _) _ _] => intros; apply FixList_decode_correct
+
+  | |- appcontext [encode_decode_correct_f _ _ _ _ (encode_bool_Spec) _ _] =>
+    apply bool_decode_correct
+
+  | |- appcontext [encode_decode_correct_f _ _ _ _ (encode_option_Spec _ _) _ _] =>
+    intros; eapply option_encode_correct;
+    [ match goal with
+        H : cache_inv_Property _ _ |- _ => eexact H
+        end | .. ]
+
   | |- appcontext [encode_decode_correct_f _ _ _ _ (encode_enum_Spec _) _ _] =>
     eapply Enum_decode_correct
-  (* C) Discharging a side condition of one of the base rules *)
+
+  | |- appcontext[encode_decode_correct_f _ _ _ _ encode_string_Spec _ _ ] =>
+    eapply String_decode_correct
+  | |- appcontext [encode_decode_correct_f _ _ _ _ (encode_SumType_Spec (B := ?B) (cache := ?cache) (m := ?n) ?types _) _ _] =>
+    let cache_inv_H := fresh in
+    intros cache_inv_H;
+      first
+        [let types' := (eval unfold types in types) in
+         ilist_of_evar
+           (fun T : Type => T -> @CacheEncode cache -> Comp (B * @CacheEncode cache))
+           types'
+           ltac:(fun encoders' =>
+         ilist_of_evar
+           (fun T : Type => B -> @CacheDecode cache -> option (T * B * @CacheDecode cache))
+           types'
+           ltac:(fun decoders' =>
+         ilist_of_evar
+           (fun T : Type => Ensembles.Ensemble T)
+           types'
+           ltac:(fun invariants' =>
+         ilist_of_evar
+            (fun T : Type => T -> B -> Prop)
+           types'
+           ltac:(fun invariants_rest' =>
+         Vector_of_evar
+           n
+           (Ensembles.Ensemble (CacheDecode -> Prop))
+         ltac:(fun cache_invariants' =>
+                       eapply (SumType_decode_correct (m := n) types) with
+                   (encoders := encoders')
+                     (decoders := decoders')
+                     (invariants := invariants')
+                     (invariants_rest := invariants_rest')
+                     (cache_invariants :=  cache_invariants')
+                )))))
+        |          ilist_of_evar
+           (fun T : Type => T -> @CacheEncode cache -> Comp (B * @CacheEncode cache))
+           types
+           ltac:(fun encoders' =>
+         ilist_of_evar
+           (fun T : Type => B -> @CacheDecode cache -> option (T * B * @CacheDecode cache))
+           types
+           ltac:(fun decoders' =>
+         ilist_of_evar
+           (fun T : Type => Ensembles.Ensemble T)
+           types
+           ltac:(fun invariants' =>
+          ilist_of_evar
+            (fun T : Type => T -> B -> Prop)
+           types
+           ltac:(fun invariants_rest' =>
+         Vector_of_evar
+           n
+           (Ensembles.Ensemble (CacheDecode -> Prop))
+           ltac:(fun cache_invariants' =>
+                       eapply (SumType_decode_correct (m := n) types) with
+                   (encoders := encoders')
+                     (decoders := decoders')
+                     (invariants := invariants')
+                     (invariants_rest := invariants_rest')
+                     (cache_invariants :=  cache_invariants'))))))
+        ];
+      [ simpl; repeat (apply Build_prim_and; intros); try exact I
+      | apply cache_inv_H ]
+        (* C) Discharging a side condition of one of the base rules *)
   | |- NoDupVector _ => Discharge_NoDupVector
   | |- context[Vector_predicate_rest (fun _ _ => True) _ _ _ _] =>
     intros; apply Vector_predicate_rest_True
   | _ => solve [solve_data_inv]
+  | _ => solve [intros; instantiate (1 := fun _ _ => True); exact I]
   (* D) Solving the goal once all the byte string has been parsed *)
   | _ =>  solve [simpl; intros;
                  eapply encode_decode_correct_finish;
@@ -171,8 +363,8 @@ Ltac synthesize_decoder :=
     [ repeat decode_step
     | cbv beta; synthesize_cache_invariant ].
 
-
-
+Global Instance : DecideableEnsembles.Query_eq () :=
+  {| A_eq_dec a a' := match a, a' with (), () => left (eq_refl _) end |}.
 
 (* Older tactics follow, leaving in for now for backwards compatibility. *)
 
